dist/gcc-compatible/lib/Hacl_Streaming_HMAC_bindings.ml
@@ -91,9 +91,9 @@ module Bindings(F:Cstubs.FOREIGN) =
     let _ = seal hacl_Streaming_HMAC_agile_state
     let hacl_Streaming_HMAC_malloc =
       foreign "Hacl_Streaming_HMAC_malloc"
-        (hacl_Streaming_HMAC_Definitions_index @->
-           (hacl_Streaming_HMAC_Definitions_key_and_len @->
-              (returning (ptr hacl_Streaming_HMAC_agile_state))))
+        (hacl_Agile_Hash_impl @->
+           (ocaml_bytes @->
+              (uint32_t @-> (returning (ptr hacl_Streaming_HMAC_agile_state)))))
     let hacl_Streaming_HMAC_reset =
       foreign "Hacl_Streaming_HMAC_reset"
         ((ptr hacl_Streaming_HMAC_agile_state) @->
